examples/sgx/Ast.fst
@@ -5,12 +5,13 @@ open FStar.UInt64
 
 open Helper
 
+exception Halt
 let u32 = UInt32.t
 let u64 = UInt64.t
 
 type exp =
- |Reg of string
- |Constant of u64
+ |RegExp of string
+ |ConstantExp of u64
 
 type stmt = 
  |Store of exp * exp
@@ -29,5 +30,26 @@ type sgxmem =
 | Register of string
 | Memory of u64
 
-val lookup: (sgxmem->u64)->sgxmem -> u64
-val extend: (sgxmem -> u64)->sgxmem->u64 ->(sgxmem->u64)
+
+type lowexp =
+ |LowVarExp of string
+ |LowConstantExp of u64
+ |LowMemExp of u64
+
+type lowstmt = 
+ |LowStore of lowexp * lowexp
+ |LowAssign of lowexp * lowexp
+ |LowLoad of lowexp * lowexp
+ |LowSeq of (list lowstmt)
+ |LowIf of lowexp * (list lowstmt) * (list lowstmt)
+ |LowJump of lowexp
+ |LowCall of lowexp
+ |LowSkip 
+ |LowAssert
+
+type lowprogram = lowstmt
+
+type lowsgxmem = 
+| LowRegister of string
+| LowMemory of u64
+
