examples/sgx/Helper.fst
@@ -1,6 +1,87 @@
 module Helper
 open FStar.UInt64
+open FStar.Buffer 
 
 let int_of_string s = of_string s
 
+
+let u32 = UInt32.t
+let u64 = UInt64.t
+
+(* Some random values for now, the information should actually come
+ from parsing low* and assembly manifests
+*)
+let lowsgxmemorysize:u32 = 4096ul
+let lowsgxmemory = create 0uL lowsgxmemorysize
+ 
+
+let sgxbitmapaddr:u64 = 0x0uL
+let sgxuheapaddr:u64 = 0x0uL 
+let sgxustackaddr:u64 = 0x0uL 
+let sgxucodeaddr:u64 = 0x0uL 
+let sgxucodesize:u64  = 0x0uL
+
+let lowsgxmemstart = 0x0uL
+let lowsgxbitmapoffset = lowsgxmemstart 
+let lowsgxuheapoffset = 0x0uL 
+let lowsgxustackoffset = 0x0uL 
+let lowsgxustacksize = 0x0uL 
+
+(* Functions determining if assembly address falls in one of the regions
+ *)
+val issgxaddrinbitmap: u64 -> bool
+let issgxaddrinbitmap sgxaddr = 
+ if (lt sgxaddr sgxuheapaddr) && (gt sgxaddr sgxbitmapaddr) then
+	true
+ else
+	false
+	  
+val issgxaddrinuheap: u64 -> bool
+let issgxaddrinuheap sgxaddr = 
+ if (lt sgxaddr sgxustackaddr) && (gt sgxaddr sgxuheapaddr) then
+	true
+ else
+	false
+
+val issgxaddrinustack: u64 -> bool
+let issgxaddrinustack sgxaddr = 
+ if (lt sgxaddr sgxucodeaddr) && (gt sgxaddr sgxustackaddr) then
+	true
+ else
+	false
+
+	  
+val issgxaddrinucode: u64 -> bool
+let issgxaddrinucode sgxaddr = 
+ if (gt sgxaddr sgxucodeaddr) && (lt sgxaddr (add sgxucodeaddr sgxucodesize)) then
+	true
+ else
+	false
+
+(* Functions determining if low* offset falls in 
+  one of the low* memory regions
+ *)
+val islowsgxoffsetinbitmap: u64 -> bool
+let islowsgxoffsetinbitmap lowsgxoffset = 
+ if (lt lowsgxoffset lowsgxuheapoffset) && (gt lowsgxoffset lowsgxbitmapoffset) then
+	true
+ else
+	false
+	  
+val islowsgxoffsetinuheap: u64 -> bool
+let islowsgxoffsetinuheap lowsgxoffset = 
+ if (lt lowsgxoffset lowsgxustackoffset) && (gt lowsgxoffset lowsgxuheapoffset) then
+	true
+ else
+	false
+
+val islowsgxoffsetinustack: u64 -> bool
+let islowsgxoffsetinustack lowsgxoffset = 
+ if (lt lowsgxoffset (add lowsgxustackoffset  lowsgxustacksize)) && (gt lowsgxoffset lowsgxustackoffset) then
+	true
+ else
+	false
+
+	  
+(* Support for code section *)
 
