examples/sgx/X86Interpreter.fst
@@ -6,37 +6,61 @@ open FStar.HST
 open FStar.Int.Cast
 open FStar.UInt64
 open FStar.Buffer
-open Ast
 open FStar.List
+open Ast
+open LowInterpreter
+open Helper
+open Prims
 
-exception Halt
 
+val lookup: (sgxmem->u64)->sgxmem -> u64
+val extend: (sgxmem -> u64)->sgxmem->u64 ->(sgxmem->u64)
 (* Fix these definitions *)
 let lookup sgxenv key =  sgxenv key
 let extend sgxenv key value = sgxenv
 let get_register_string r = 
 	begin match r with
-	|Reg rs -> rs
+	|RegExp rs -> rs
 	|_ -> raise Halt
 	end 
 
+
+(* Takes in an assembly address and converts it to low* offset *)
+let translate_address sgxaddr= 
+ 	let tmp = (FStar.UInt64.sub sgxaddr sgxbitmapaddr) in
+ 	LowMemExp tmp
+
+let translate_reg e = match e with
+ | RegExp r -> LowVarExp r
+ | ConstantExp n -> LowConstantExp n 
+
 val interpret_exp: exp -> (sgxmem->u64) -> u64
 let interpret_exp e (sgxenv: sgxmem->u64) = begin match e with
- | Reg r -> lookup sgxenv (Register r)
- | Constant u -> u
+ | RegExp r -> lookup sgxenv (Register r)
+ | ConstantExp u -> u
 end
 
-val interpret: stmt -> (sgxmem->u64) -> (sgxmem->u64)
-let rec interpret progstmt (sgxenv: sgxmem->u64) = begin match progstmt with
-  | Skip -> sgxenv 
-  | Store(ea, ed)-> let lea = interpret_exp ea sgxenv in
-		     let leb = interpret_exp ed sgxenv  in
-		     extend sgxenv (Memory lea) leb  
-  | Load(r, ea)-> let lea = interpret_exp ea sgxenv in
-		    let v = lookup sgxenv (Memory lea) in
+val interpret: stmt -> (sgxmem->u64) -> (lowsgxmem->u64) ->((sgxmem->u64)*(lowsgxmem->u64))
+let rec interpret (progstmt:stmt) (sgxenv:sgxmem->u64) (lowsgxenv:lowsgxmem->u64) = begin match progstmt with
+  | Skip -> (sgxenv, lowsgxenv)
+  | Store(ea, ed)-> let vea = interpret_exp ea sgxenv in
+		    let ved = interpret_exp ed sgxenv  in
+		    let sgxenv' = extend sgxenv (Memory vea) ved  in
+
+		    let lea = translate_address vea in
+		    let led = translate_reg ed in
+		    let lowsgxenv' = low_interpret (LowStore (lea, led)) lowsgxenv in	
+		    (sgxenv', lowsgxenv')
+  | Load(r, ea)->   let vea = interpret_exp ea sgxenv in
+		    let v = lookup sgxenv (Memory vea) in
 		    let rs = get_register_string r in
-		    extend sgxenv (Register rs) v  
-  | Seq(li) -> fold_left (fun sgxenv elem ->interpret elem sgxenv) sgxenv li 
-  | _   -> sgxenv
+		    let sgxenv' = extend sgxenv (Register rs) v  in
+
+		    let lea = translate_address vea in
+		    let lr = translate_reg r in
+		    let lowsgxenv' = low_interpret (LowLoad (lr, lea)) lowsgxenv in	
+		    (sgxenv', lowsgxenv')
+  | Seq(li) -> fold_left (fun envpair elem ->interpret elem (fst envpair) (snd envpair)) (sgxenv, lowsgxenv) li 
+  | _   ->(sgxenv, lowsgxenv)
 end
 
