examples/sgx/LowInterpreter.fst
@@ -1,0 +1,39 @@
+module LowInterpreter 
+
+open Ast
+open FStar.UInt64
+open FStar.Buffer 
+open FStar.List
+
+let u64 = UInt64.t
+
+val lowlookup: (lowsgxmem->u64)->lowsgxmem -> u64
+val lowextend: (lowsgxmem -> u64)->lowsgxmem->u64 ->(lowsgxmem->u64)
+
+(* Fix these definitions *)
+let lowlookup lowsgxenv key =  lowsgxenv key
+let lowextend lowsgxenv key value = lowsgxenv
+
+let get_var_string r = 
+	begin match r with
+	|LowVarExp vs -> vs
+	|_ -> raise Halt
+	end 
+
+let rec low_interpret_exp  le lowsgxenv = match le with 
+ | LowVarExp v -> lowlookup lowsgxenv (LowRegister v)
+ | LowMemExp offset -> lowlookup lowsgxenv (LowMemory offset)
+ | LowConstantExp n -> n
+
+let rec low_interpret progstmt lowsgxenv = match progstmt with 
+  | LowSkip -> lowsgxenv 
+  | LowStore(lea, led)-> let vea = low_interpret_exp lea lowsgxenv in
+		     let veb = low_interpret_exp led lowsgxenv  in
+		     lowextend lowsgxenv (LowMemory vea) veb  
+  | LowLoad(lv, lea)-> let vea = low_interpret_exp lea lowsgxenv in
+		    let value = lowlookup lowsgxenv (LowMemory vea) in
+		    let vs = get_var_string lv in
+		    lowextend lowsgxenv (LowRegister vs) value  
+  | LowSeq(li) -> fold_left (fun lowsgxenv elem ->low_interpret elem lowsgxenv) lowsgxenv li 
+  | _   -> lowsgxenv
+
